theories/IO_Axioms.v
@@ -1,0 +1,28 @@
+(** Abstract definitions of IO Stub signatures.  Functions with monadic 
+    return types (i.e. do_start_par_thread) should be replaced by concrete monadic 
+    functions in the target language upon extraction.  Alternatively,
+    if the target language does not have built-in monadic support, one can
+    instantiate a non-monadic version of the stub instead.
+
+    The non-monadic stubs (i.e. doRemote_uuid) remain abstract (Admitted) in Coq 
+    because they are either too low-level to reason about, or require external 
+    IO capabilities not modeled first-class in our spec.  The abstract binary
+    and EvidenceT value results support specification of correctness properties 
+    for Appraisal.        
+ *)
+From CoplandSpec Require Import Term_Defs.
+From RocqCandy Require Import StateMonad.
+From CVM Require Import Attestation_Session St.
+
+Definition make_JSON_Network_Request (uuid : IP_Port) (js : JSON) : Result JSON string. Admitted.
+
+Definition aspid_to_fs_location (aspid : ASP_ID) : FS_Location. Admitted.
+
+Definition make_JSON_FS_Location_Request (dir : FS_Location) (aspid : FS_Location) (js : JSON) : Result JSON string. Admitted.
+
+(** * Stub to simulate EvidenceT collected by a parallel CVM instance *)
+Definition parallel_vm_thread (l:Loc) (p:Plc) (e:Evidence) (t: Term) : Result Evidence CVM_Error.  Admitted.
+
+Definition do_start_par_thread (loc:Loc) (e: Evidence) (t: Term) : CVM unit :=
+  ret tt.
+
