theories/Impl.v
@@ -8,7 +8,8 @@
 *)
 
 From RocqCandy Require Import All.
-Require Import Term_Defs Cvm_Monad.
+From CoplandSpec Require Import Term_Defs.
+From CVM Require Import Monad.
 
 (** Monadic CVM implementation (top-level) *)
 Fixpoint build_cvm (e : Evidence) (t: Term) : CVM Evidence :=
@@ -16,21 +17,21 @@ Fixpoint build_cvm (e : Evidence) (t: Term) : CVM Evidence :=
   | asp a => do_prim e a 
   | att q t' => doRemote q e t'
   | lseq t1 t2 =>
-    e1 <- build_cvm e t1 ;;
+    e1 <~ build_cvm e t1 ;;;
     build_cvm e1 t2
 
   | bseq s t1 t2 =>
-    split_ev ;;
-    e1r <- build_cvm (splitEv_l s e) t1 ;;
-    e2r <- build_cvm (splitEv_r s e) t2 ;;
+    split_ev ;;;
+    e1r <~ build_cvm (splitEv_l s e) t1 ;;;
+    e2r <~ build_cvm (splitEv_r s e) t2 ;;;
     join_seq e1r e2r
 
   | bpar s t1 t2 =>
-    split_ev ;;
+    split_ev ;;;
     (* We will make the LOC = event_id for start of thread *)
     (* start a parallel thread working on the evidence split for t2 *)
-    loc <- start_par_thread (splitEv_r s e) t2 ;;
-    e1r <- build_cvm (splitEv_l s e) t1 ;;
-    e2r <- wait_par_thread loc (splitEv_r s e) t2 ;;
+    loc <~ start_par_thread (splitEv_r s e) t2 ;;;
+    e1r <~ build_cvm (splitEv_l s e) t1 ;;;
+    e2r <~ wait_par_thread loc (splitEv_r s e) t2 ;;;
     join_seq e1r e2r
   end.
