theories/Interface/Interface.v
@@ -1,0 +1,1 @@
+From CVM.Interface Require Export Interface_Types Interface_JSON.
