theories/Interface/Interface_Types.v
@@ -1,0 +1,44 @@
+From RocqJSON Require Import JSON.
+From CoplandSpec Require Import Term_Defs.
+From CVM Require Import Attestation_Session.
+
+(* Interface Types *)
+Record ProtocolRunRequest := 
+  mkPRReq {
+    prreq_att_sess : Attestation_Session;
+    prreq_req_plc: Plc;
+    prreq_Evidence: Evidence;
+    prreq_term: Term;
+  }.
+
+Record ProtocolRunResponse := 
+  mkPRResp {
+    prresp_success: bool;
+    prresp_Evidence: Evidence;
+  }.
+
+Record ProtocolNegotiateRequest := 
+  mkPNReq {
+    pnreq_term: Term;
+  }.
+
+Record ProtocolNegotiateResponse := 
+  mkPNResp {
+    pnresp_success: bool;
+    pnresp_term: Term;
+  }.
+
+Record ASPRunRequest := 
+  mkASPRReq {
+    asprreq_asp_id : ASP_ID;
+    asprreq_asp_args: ASP_ARGS;
+    asprreq_targ_plc : Plc ;
+    asprreq_targ : TARG_ID ;
+    asprreq_rawev : RawEv;
+  }.
+
+Record ASPRunResponse := 
+  mkASPRResp {
+    asprresp_success: bool;
+    asprresp_rawev: RawEv;
+  }.
