theories/Monad.v
@@ -1,0 +1,459 @@
+(*
+  Definition of the CVM Monad + monadic helper functions.
+  Also included:  core simplification/automation tactics for the CVM Monad.
+
+  Author:  Adam Petz, ampetz@ku.edu
+*)
+From CoplandSpec Require Import Term_Defs Event_System.
+
+From CVM Require Export Attestation_Session St IO_Axioms Utils.
+From CVM Require Import Interface.Interface.
+
+(** * CVM monadic primitive operations *)
+
+Definition get_st : CVM cvm_st :=
+  st_conf <~ get ;;;
+  match st_conf with
+  | (st, conf) => ret st
+  end.
+
+Definition get_config : CVM Session_Config :=
+  st_conf <~ get ;;;
+  match st_conf with
+  | (st, conf) => ret conf
+  end.
+
+Definition get_trace : CVM (list Ev) :=
+  st <~ get_st ;;;
+  ret (st_trace st).
+
+Definition get_evid : CVM Event_ID :=
+  st <~ get_st ;;;
+  ret (st_evid st).
+
+Definition put_trace (tr' : list Ev) : CVM unit :=
+  i <~ get_evid ;;;
+  conf <~ get_config ;;;
+  put (mk_st tr' i, conf).
+
+Definition put_evid (i' : Event_ID) : CVM unit :=
+  tr <~ get_trace ;;;
+  conf <~ get_config ;;;
+  put (mk_st tr i', conf).
+
+Definition get_pl : CVM Plc :=
+  sc <~ get_config ;;;
+  ret (session_plc sc).
+
+Definition inc_id : CVM Event_ID :=
+  tr <~ get_trace ;;;
+  i <~ get_evid ;;;
+  conf <~ get_config ;;;
+  put (mk_st tr (Nat.add i 1), conf) ;;;
+  ret i.
+
+Definition add_trace (tr:list Ev) : CVM unit :=
+  tr' <~ get_trace ;;;
+  put_trace (tr' ++ tr).
+
+(* TODO: consider removing split/join events from reference semantics.
+         Would make this (no-op) helper unecessary. *)
+Definition split_ev : CVM unit :=
+  p <~ get_pl ;;;
+  i <~ inc_id ;;;
+  add_trace [Term_Defs.split i p].
+
+(** * Partially-symbolic implementations of IO operations *)
+
+(* Generates a new event ID and adds a measurement event with that ID to the 
+   CVM internal trace.  Returns the new Event_ID (used to represent raw 
+   EvidenceT, relevant for appraisal verification).  *)
+Definition tag_ASP (params :ASP_PARAMS) (mpl:Plc) (e:Evidence) : CVM Event_ID :=
+  x <~ inc_id ;;;
+  add_trace [umeas x mpl params (get_et e)] ;;;
+  ret x.
+
+Local Open Scope list_scope.
+
+Definition join_seq (e1:Evidence) (e2:Evidence): CVM Evidence :=
+  p <~ get_pl ;;;
+  n <~ inc_id ;;;
+  let '(evc bits1 et1) := e1 in
+  let '(evc bits2 et2) := e2 in
+  add_trace [join n p] ;;;
+  ret (evc (bits1 ++ bits2) (split_evt et1 et2)).
+
+Definition hoist_result {A : Type} (r : Result A string) : CVM A :=
+  match r with
+  | res a => ret a
+  | err e => fail (dispatch_error (Runtime e))
+  end.
+
+Definition hoist_option {A : Type} (o : option A) (msg : string) : CVM A :=
+  match o with
+  | Some a => ret a
+  | None => fail (dispatch_error (Runtime msg))
+  end.
+
+Definition get_asp_type (a : ASP_ID) : CVM EvSig :=
+  sc <~ get_config ;;;
+  let G := session_context sc in
+  hoist_option ((asp_types G) ![ a ]) err_str_asp_no_type_sig.
+
+Definition get_asp_dual (a : ASP_ID) : CVM ASP_ID :=
+  sc <~ get_config ;;;
+  let G := session_context sc in
+  hoist_option ((asp_comps G) ![ a ]) err_str_asp_no_compat_appr_asp.
+
+(* Helper function that builds a new internal EvidenceT bundle based on 
+   the EvidenceT extension parameter of an ASP term. *)
+Definition bundle_asp (p:Plc) (rwev : RawEv) 
+    (cur_ev : Evidence) (ps:ASP_PARAMS) : CVM Evidence :=
+  let '(asp_paramsC asp_id args targ_plc targ) := ps in
+  '(ev_arrow fwd in_sig out_sig) <~ get_asp_type asp_id ;;;
+  match out_sig with
+  | (OutN n) =>
+    if (dec_eq (List.length rwev) n)
+    then 
+      match fwd with
+(* The semantics for a "REPLACE" asp are it CONSUMES all incoming evidence,
+then returns a new collection of evidence that will REPLACE the CVMs current 
+Evidence *)
+      | REPLACE => ret (evc rwev (asp_evt p ps (get_et cur_ev)))
+(* The semantics for a "WRAP" asp are the exact same as "REPLACE" for the 
+attestation and bundling side of the CVM. Wraps main distinction lies in the
+fact that its is a GUARANTEE, that the dual appraisal ASP is actually an
+inverse, thus allowing WRAPPED evidence to be recovered via appraisal *)
+      | WRAP => ret (evc rwev (asp_evt p ps (get_et cur_ev)))
+      | UNWRAP => fail (dispatch_error (Runtime err_str_unwrap_must_have_outwrap))
+(* The semantics for an "EXTEND" asp are it APPENDS all incoming evidence to the
+current CVM evidence bundle *)
+      | EXTEND =>
+        match cur_ev with
+        | evc bits et => ret (evc (rwev ++ bits) (asp_evt p ps et))
+        end
+      end
+    else fail (dispatch_error (Runtime errStr_raw_EvidenceT_too_long))
+  | OutUnwrap =>
+    match fwd with
+    | WRAP => fail (dispatch_error (Runtime err_str_only_unwrap_can_be_outwrap))
+    | REPLACE => fail (dispatch_error (Runtime err_str_only_unwrap_can_be_outwrap))
+    | EXTEND => fail (dispatch_error (Runtime err_str_only_unwrap_can_be_outwrap))
+    | UNWRAP => 
+      sc <~ get_config ;;;
+      let G := (session_context sc) in
+      let '(evc bits et) := cur_ev in
+      size_below_wrap' <~ hoist_result (apply_to_evidence_below G (et_size G) [Trail_UNWRAP asp_id] et) ;;;
+      size_below_wrap <~ hoist_result (size_below_wrap' ) ;;;
+      (* we now need to just verify that we are the same size as what was below the wrap *)
+      if (dec_eq (List.length rwev) size_below_wrap)
+      then ret (evc rwev (asp_evt p ps et))
+      else fail (dispatch_error (Runtime err_str_unwrap_of_wrap_same_size))
+      (* match r with
+      | asp_evt p' (asp_paramsC wrap_id _ _ _) et' =>
+        '(ev_arrow fwd _ _) <~ get_asp_type wrap_id ;;;
+        match fwd with
+        | WRAP =>
+          (* we are an UNWRAP or a WRAP, so new size is the sizer of et' *)
+          match et_size G et' with
+          | errC e => fail (dispatch_error (Runtime e))
+          | resultC et'_size =>
+            if (eqb (length rwev) et'_size)
+            then (* we are the right inverse size! *)
+              ret (evc rwev (asp_evt p ps et))
+            else fail (dispatch_error (Runtime err_str_unwrap_of_wrap_same_size))
+          end
+        | _ => fail (dispatch_error (Runtime err_str_unwrap_only_wrap))
+        end
+      | _ => fail (dispatch_error (Runtime err_str_unwrap_only_wrap))
+      end *)
+    end
+  end.
+
+(** * Stub for invoking external ASP procedures.  
+      Extracted code should not need to use the Plc or Event_ID parameters 
+      (those can be erased upon extraction). *)
+Definition do_asp (params :ASP_PARAMS) (e:RawEv) (x:Event_ID) : CVM RawEv :=
+  sc <~ get_config  ;;;
+  match (sc.(asp_cb) params e) with
+  | res r => ret r
+  | err e => fail (dispatch_error e)
+  end.
+
+(* Simulates invoking an arbitrary ASP.  Tags the event, builds and returns 
+   the new EvidenceT bundle. *)
+Definition invoke_ASP (e : Evidence) (params : ASP_PARAMS) : CVM Evidence :=
+  p <~ get_pl ;;;
+  x <~ tag_ASP params p e ;;;
+  rawev <~ do_asp params (get_bits e) x ;;;
+  outev <~ bundle_asp p rawev e params ;;;
+  ret outev.
+
+(* Simulates invoking an arbitrary ASP.  Tags the event, builds and returns 
+   the new EvidenceT bundle. *)
+
+Fixpoint invoke_APPR' (r : RawEv) (et : EvidenceT) (out_evt : EvidenceT) {struct et} : CVM Evidence :=
+  sc <~ get_config ;;;
+  let G := (session_context sc) in
+  match et with
+  | mt_evt => ret mt_evc 
+  | nonce_evt n' => invoke_ASP (evc r out_evt) check_nonce_params
+  | asp_evt p' par et' =>
+    let '(asp_paramsC asp_id args targ_plc targ) := par in
+    appr_asp_id <~ get_asp_dual asp_id ;;;
+    let dual_par := asp_paramsC appr_asp_id args targ_plc targ in
+    '(ev_arrow fwd in_sig out_sig) <~ get_asp_type asp_id ;;;
+    match fwd with
+    | REPLACE => (* Only do the dual ASP *)
+      invoke_ASP (evc r out_evt) dual_par
+    | WRAP =>
+      (* first do the dual ASP to unwrap *)
+      (* NOTE: Do we need to be checking that appr_asp_id is an UNWRAP here? *)
+      '(evc r'' et'') <~ invoke_ASP (evc r out_evt) dual_par ;;;
+      (* Check that the "UNWRAP" occured properly *)
+      n' <~ hoist_result (et_size G et'') ;;;
+      n'' <~ hoist_result (et_size G et') ;;;
+      if (dec_eq n' n'')
+      then (* The "UNWRAP" worked *)
+        (* so do the recursive call *)
+        invoke_APPR' r'' et' (asp_evt (session_plc sc) dual_par out_evt)
+      else fail (dispatch_error (Runtime err_str_appr_wrap_failed))
+    | UNWRAP =>
+      (* to appraise an UNWRAP is to appraise whatever is below 
+      the UNWRAP and WRAP *)
+      match out_sig with
+      | OutN _ => fail (dispatch_error (Runtime err_str_unwrap_must_have_outwrap)) 
+      | OutUnwrap =>
+        e <~ hoist_result (apply_to_evidence_below G (fun e => invoke_APPR' r e out_evt) [Trail_UNWRAP asp_id] et') ;;;
+        e 
+        (* e <- hoist_result (
+          apply_to_asp_under_wrap G asp_id (fun e => invoke_APPR' r e out_evt) et'
+        ) ;;
+        e *)
+      end
+
+    | EXTEND =>
+      match out_sig with
+      | OutUnwrap => fail (dispatch_error (Runtime err_str_extend_must_have_outn))
+      | (OutN n) =>
+        (* first we split, left for the appr of extended part, right for rest *)
+        split_ev ;;;
+        '(_, r_ev) <~ (hoist_result (peel_n_rawev n r)) ;;;
+
+        (* on left we do the dual of EXTEND *)
+        ev1 <~ invoke_ASP (evc r out_evt) dual_par ;;;
+
+        (* now on right, we work only on the remaining evidence *)
+        (* our new evidence is e' *)
+        (* now we do the recursive call *)
+        ev2 <~ invoke_APPR' r_ev et' et' ;;;
+        (* now join *)
+        join_seq ev1 ev2 
+      end
+      (* ev' <~ invoke_ASP (asp_paramsC appr_asp_id args targ_plc targ) ;;;
+      put_ev ev' *)
+    end
+  | left_evt et' =>
+    r <~ hoist_result (apply_to_evidence_below G (fun e => invoke_APPR' r e out_evt) [Trail_LEFT] et') ;;;
+    r
+
+  | right_evt et' =>
+    r <~ hoist_result (apply_to_evidence_below G (fun e => invoke_APPR' r e out_evt) [Trail_RIGHT] et') ;;;
+    r
+
+  | split_evt et1 et2 =>
+    n1 <~ hoist_result (et_size G et1) ;;;
+    n2 <~ hoist_result (et_size G et2) ;;;
+    '(ev_l, r_ev) <~ (hoist_result (peel_n_rawev n1 r)) ;;;
+    '(ev_r, rest) <~ (hoist_result (peel_n_rawev n2 r_ev)) ;;;
+    match rest with
+    | [] => 
+      if (equiv_EvidenceT G et1 (left_evt out_evt))
+      then if (equiv_EvidenceT G et2 (right_evt out_evt))
+      then
+        split_ev ;;; (* register event that we are splitting evidence *)
+        (* first we must get out the actual Evidence for et1 *)
+        ev1 <~ invoke_APPR' ev_l et1 (left_evt out_evt) ;;;
+        ev2 <~ invoke_APPR' ev_r et2 (right_evt out_evt) ;;;
+        join_seq ev1 ev2
+      else fail (dispatch_error (Runtime err_str_ev_split_failed_not_empty))
+      else fail (dispatch_error (Runtime err_str_ev_split_failed_not_empty))
+      (* ev1 <~ invoke_APPR' ev_l et1 (left_evt out_evt) ;;;
+      ev2 <~ invoke_APPR' ev_r et2 (right_evt out_evt) ;;;
+      join_seq ev1 ev2 *)
+    | _ => fail (dispatch_error (Runtime err_str_ev_split_failed_not_empty))
+    end
+  end.
+
+Definition invoke_APPR (e : Evidence) : CVM Evidence :=
+  invoke_APPR' (get_bits e) (get_et e) (get_et e).
+
+Definition nullEv : CVM Evidence :=
+  p <~ get_pl ;;;
+  x <~ inc_id ;;;
+  add_trace [null x p] ;;;
+  ret mt_evc.
+
+Definition clearEv : unit -> CVM Evidence :=
+  fun _ => ret mt_evc.
+
+(* Helper that interprets primitive core terms in the CVM.  *)
+Definition do_prim (e : Evidence) (a: ASP) : CVM Evidence :=
+  match a with
+  | NULL => nullEv
+  | ASPC params => invoke_ASP e params
+  | SIG => invoke_ASP e sig_params
+  | HSH => invoke_ASP e hsh_params
+  | APPR => invoke_APPR e 
+  | ENC q => invoke_ASP e (enc_params q)
+  end.
+
+(* Monadic helper function to simulate a span of remote event IDs 
+   corresponding to the size of a Term *)
+Definition inc_remote_event_ids (e : Evidence) (t:Term) : CVM unit :=
+  i <~ get_evid ;;;
+  sc <~ get_config ;;;
+  p <~ get_pl ;;;
+  n <~ hoist_result (events_size (session_context sc) p (get_et e) t) ;;;
+  put_evid (Nat.add i n).
+
+(* Monadic helper function to simulate a span of parallel event IDs 
+   corresponding to the size of a Term *)
+Definition inc_par_event_ids (e : Evidence) (t: Term) : CVM unit :=
+  i <~ get_evid ;;;
+  sc <~ get_config ;;;
+  p <~ get_pl ;;;
+  n <~ hoist_result (events_size (session_context sc) p (get_et e) t) ;;;
+  put_evid (Nat.add i n).
+  
+(* Primitive monadic communication primitives 
+   (some rely on Admitted IO Stubs). *)
+
+Definition tag_REQ (t:Term) (p:Plc) (q:Plc) (e:Evidence) : CVM unit :=
+  reqi <~ inc_id ;;;
+  add_trace [req reqi p q (get_et e) t].
+
+Definition tag_RPY (p:Plc) (q:Plc) (e:Evidence) : CVM unit :=
+  rpyi <~ inc_id ;;;
+  add_trace [rpy rpyi p q (get_et e)].
+
+Definition get_cvm_policy : CVM PolicyT := 
+  sc <~ get_config ;;;
+  ret (policy sc).
+
+(* Remote communication primitives *)
+
+Definition do_remote (sc : Session_Config) (pTo: Plc) (e : Evidence) (t:Term) 
+    : Result Evidence CVM_Error := 
+  (* There is assuredly a better way to do it than this *)
+  let '(mkAtt_Sess my_plc plc_map pk_map G) := (session_config_decompiler sc) in
+  (* We need  to update the Att Session to tell the next plc how
+  they should be tagging their stuff (basically who they are
+  in the protocol) *)
+  let new_att_sess := (mkAtt_Sess pTo plc_map pk_map G) in
+  match (plc_map ![ pTo ]) with 
+  | Some IP_Port => 
+      let remote_req := (mkPRReq new_att_sess my_plc e t) in
+      let js_req := to_JSON remote_req in
+      let resp_res := make_JSON_Network_Request IP_Port js_req in
+      match resp_res with
+      | res js_resp =>
+          match from_JSON js_resp with
+          | res resp => 
+              let '(mkPRResp success ev) := resp in
+              if success 
+              then res ev 
+              else err (dispatch_error (Runtime errStr_remote_am_failure))
+          | err msg => err (dispatch_error (Runtime msg)) 
+          end
+      | err msg => err (dispatch_error (Runtime msg))
+      end
+  | None => err (dispatch_error Unavailable)
+  end.
+
+Definition doRemote_session' (pTo:Plc) (e:Evidence) (t:Term) 
+    : CVM Evidence := 
+  sc <~ get_config ;;;
+  (* We need to check that the policy allows us to do this remote call *)
+  match (do_remote sc pTo e t) with
+  | res e' => ret e'
+  | err s => fail s
+  end.
+
+Definition remote_session (p:Plc) (q:Plc) (e:Evidence) (t:Term) : CVM Evidence :=
+  tag_REQ t p q e ;;;
+  e' <~ doRemote_session' q e t ;;;
+  sc <~ get_config ;;;
+  i <~ get_evid ;;;
+  rem_evs <~ match events_fix (session_context sc) q (get_et e) t i with
+  | err e => fail (dispatch_error (Runtime e))
+  | res evs => ret evs
+  end ;;;
+  add_trace rem_evs ;;;
+  inc_remote_event_ids e t ;;;
+  ret e'.
+
+Definition doRemote (q:Plc) (e:Evidence) (t:Term) : CVM Evidence :=
+  p <~ get_pl ;;;
+  e' <~ remote_session p q e t ;;;
+  tag_RPY p q e' ;;;
+  ret e'.
+
+(* Primitive monadic parallel CVM thread primitives 
+   (some rely on Admitted IO Stubs). *)
+
+Definition start_par_thread (e:Evidence) (t: Term) : CVM nat :=
+  p <~ get_pl ;;;
+  i <~ inc_id ;;;
+  (* The loc always = the event id for the thread_start event *)
+  do_start_par_thread i e t ;;;
+  add_trace [cvm_thread_start i i p (get_et e) t] ;;;
+  ret i.
+
+Definition do_wait_par_thread (loc:Loc) (p:Plc) (e:Evidence) (t: Term) : CVM Evidence :=
+  match (parallel_vm_thread loc p e t) with
+  | res e' => ret e'
+  | err s => fail s
+  end.
+
+Definition wait_par_thread (loc:Loc) (e:Evidence) (t: Term) : CVM Evidence :=
+  p <~ get_pl ;;;
+  e' <~ do_wait_par_thread loc p e t ;;;
+  i <~ get_evid ;;;
+  sc <~ get_config ;;;
+  rem_evs <~ match events_fix (session_context sc) p (get_et e) t i with
+  | err e => fail (dispatch_error (Runtime e))
+  | res evs => ret evs
+  end ;;;
+  add_trace rem_evs ;;;
+  inc_par_event_ids e t ;;;
+  i <~ inc_id ;;;
+  add_trace [cvm_thread_end i loc] ;;;
+  ret e'.
+   
+Create HintDb cvm.
+Hint Unfold do_prim : cvm.
+Hint Unfold doRemote : cvm.
+Hint Unfold remote_session : cvm.
+Hint Unfold doRemote_session' : cvm.
+Hint Unfold invoke_ASP : cvm.
+Hint Unfold get_asp_type : cvm.
+Hint Unfold get_asp_dual : cvm.
+Hint Unfold bundle_asp : cvm.
+Hint Unfold do_asp : cvm.
+Hint Unfold clearEv : cvm.
+Hint Unfold nullEv : cvm.
+Hint Unfold hoist_result : cvm.
+Hint Unfold hoist_option : cvm.
+Hint Unfold inc_remote_event_ids : cvm.
+Hint Unfold inc_par_event_ids : cvm.
+Hint Unfold wait_par_thread : cvm.
+Hint Unfold do_wait_par_thread : cvm.
+Hint Unfold join_seq : cvm.
+Hint Unfold get_st : cvm.
+Hint Unfold get_pl : cvm.
+Hint Unfold get_evid : cvm.
+Hint Unfold put_evid : cvm.
+Hint Unfold get_config : cvm.
+Hint Unfold add_trace : cvm.
+Hint Unfold put_trace : cvm.
